\part{30/04 - Regras de Derivação}

\begin{multicols}{2}

\vspace{5mm}

\noindent%
\begin{minipage}{\linewidth}

\section{Derivação da Soma}
\begin{BM}
	(f+g)'(a) = f'(a) + g'(a)
\end{BM}\relax

\begin{flalign*}
&
	(f+g)'(a)
=	\lim_{x\to0}\frac{f(x)+g(x)-f(a)-g(a)}{x-a}
=	&\\&
=	\lim_{x\to0}
	\left(
		\frac{f(x)-f(a)}{x-a}
	+	\frac{g(x)-g(a)}{x-a}
	\right)
=	&\\&
=	f'(a) + g'(a)
&
\end{flalign*}

\end{minipage}

\vspace{5mm}

\noindent%
\begin{minipage}{\linewidth}

\section{Derivação do Produto}
\begin{BM}
	(f\,g)'(a) = f'(a)\,g(a) + f(a)\,g'(a)
\end{BM}\relax

\begin{flalign*}
&
	(f\,g)'(a)
=	\lim_{x\to a}\frac{f(x)\,g(x) - f(a)\,g(a)}{x-a}
=	&\\&
=	\lim_{x\to a}
	\frac
		{\left(f(x)-f(a)\right)\,g(x) + f(a)\left(g(x)-g(a)\right)}
		{x-a}
=	&\\&
=	\lim_{x\to a}
	\left(
		g(x)\frac{f(x)-f(a)}{x-a}
	+	f(x)\frac{g(x)-g(a)}{x-a}
	\right)
=	&\\&
=	g(x)\,f'(x)+f(x)\,g'(x)
&
\end{flalign*}

\end{minipage}

\vspace{5mm}

\noindent%
\begin{minipage}{\linewidth}

\section{Derivada da Divisão}

\subsection{Previa}
\begin{BM}
	\left( 1/f(x) \right)' = -f'(a)/f^2(a)
\end{BM}\relax

\begin{flalign*}
&
=	\lim_{x\to a}
	\frac
		{1/f(x)-1/f(a)}
		{x-a}
=	\lim_{x\to a}
	\frac
		{f(a)-f(x)}
		{(x-a)\,f(x)\,f(a)}
=	&\\&
=	-f'(a)/f^{2}(a)
&
\end{flalign*}

\end{minipage}

\vspace{5mm}

\noindent%
\begin{minipage}{\linewidth}

\section{Derivada de Conjugada}

\begin{BM}
	(f\circ u)'(a)= f'(u(a))\,u'(a)
\end{BM}\relax

\begin{flalign*}
&
	(f\circ u)'(a)
=	\lim_{x\to a}
	\frac
		{f(u(x)) - f(u(a))}
		{x-a}
=	&\\&
=	\lim_{x\to a}
	\frac
		{f(u(x))-f(u(a))}
		{u(x)-u(a)}
	\,\frac
		{u(x)-u(a)}
		{x-a}
=	f'(u(a))\,u'(a)
&
\end{flalign*}

\end{minipage}

\vspace{5mm}

\noindent%
\begin{minipage}{\linewidth}

\subsection{Exemplo}
\begin{flalign*}
&
	\left(e^{u(x)}\right)' = e^{u(x)}\,u'(x)
\qquad
	\left(e^{x^3} \right)' = e^{x^3}\,3\,x^2
&
\end{flalign*}

\end{minipage}

\vspace{5mm}

\noindent%
\begin{minipage}{\linewidth}

\subsection{Exemplo}

\paragraph{Nota:} $(\ln)'(u) = u'/u$

\begin{flalign*}
&
	\left(\ln'(1/\cos(x))\right)
=	\frac
		{-\sin(x)/x^2}
		{\cos(x)}
=	\frac{1}{\tan(x)\,x^2}
&
\end{flalign*}

\end{minipage}

\vspace{5mm}

\noindent%
\begin{minipage}{\linewidth}

\section{Tecnica de encontrar derivações}

\subsection{$\ln'(x) = 1/x$}
\begin{flalign*}
&
	\left( e^{\ln(x)} \right)' = (x)'
\implies
	e^{\ln(x)}\,\ln'(x)
=	x\,\ln'(x)
=	1
\implies &\\&
\implies
	(\ln)'(x) = 1/x
&
\end{flalign*}

\end{minipage}

\vspace{5mm}

\noindent%
\begin{minipage}{\linewidth}

\subsection{$\arctan'(x) = 1/(1+x^2)$}
\begin{flalign*}
&
	\left( \tan(\arctan(x)) \right)' = (x)'
\implies &\\&
\implies
	\tan'(\arctan(x))\,\arctan'(x)
=	&\\&
=	\left(1+\tan^2(\arctan(x))\right)\,\arctan'(x)
=	&\\&
=	\left(1+x^2\right)\,\arctan'(x)
=	1
\implies &\\&
\implies
	\arctan'(x)
=	\frac
		{1}
		{1+x^2}
&
\end{flalign*}

\end{minipage}

\vspace{5mm}

\noindent%
\begin{minipage}{\linewidth}

\subsection{$\arcsin'(x) = 1/\sqrt{1-x^2}$}
\begin{flalign*}
&
	\left(\sin(\arcsin(x))\right)' = (x)'
\implies
	\cos(\arcsin(x))\,\arcsin'(x)
=	&\\&
=	\sqrt{1-\sin^2(\arcsin(x))}\,\arcsin'(x)
=	&\\&
=	\sqrt{1-x^2}\,\arcsin'(x)
=	1
\implies
	\arcsin'(x) = 1/\sqrt{1-x^2}
&
\end{flalign*}

\end{minipage}



\end{multicols}