\part{07/05 - Resto Lagrange}

\begin{multicols}{2}

\vspace{5mm}

\noindent%
\begin{minipage}{\linewidth}

\section{Resto de Lagrange}
\begin{BM}
	f_{(\text{ord}=1,\ \text{em}=0)}=f(0)+f'(0)\,x+M_x\,x^2;
\end{BM}

\begin{flalign*}
&
	h(x)=f(x)-f(0)+f'(0)\,x+M_x\,x^2;
	& h(0)=0;
&\\&
	h'(x)=f'(x)-f'(0)+M_x\,2\,x;
	& h'(0)=0;
&\\&
	h''(x)=f''(x)-M_x\,2;
	& h'(c)=0\phantom{;}
&\\&
\implies
	M_x=f''(c)/2
&
\end{flalign*}

\end{minipage}

\begin{sectionBox}2{Exemplo}

\begin{BM}
	f(x)=\ln(x);\quad a=1
\end{BM}

\begin{flalign*}
&
	f_{(\text{ord}=1,\,\text{em}=1)}
=	\ln(1)+c^{-1}\,(x-1)
=	(x-1)/c
&\\&
	\implies
	\begin{cases}
		x>1\implies f_{(1,1)}(x)<x-1>0
	\\	x<1\implies f_{(1,1)}(x)<x-1<0
	\end{cases}
&
\end{flalign*}

\end{sectionBox}

\begin{sectionBox}2{Exemplo}

\begin{BM}
	f(x)=\arctan(x)
\end{BM}

\begin{flalign*}
&
	f_{(\text{ord}=1,\ \text{em}=0)}
=	\arctan(0)
+	(1+0^2)^{-1}(x-0)\,
+	&\\&
-	(1+c^2)^{-2}\,2*c\,(x-0)^2/2
=	x-\frac{c\,x^2}{(1+c^2)^2}
&
\end{flalign*}

\begin{flalign*}
&
	0<x<n\implies0<c<x\,\therefore x\to0^+\implies c\to0
&
\end{flalign*}

\end{sectionBox}

\begin{sectionBox}3{$
	\lim_{x\to0^+}(\arctan(x)-x)/x^2
$}
\begin{flalign*}
&
=	\lim_{x\to0^+}
	x^{-2}\,
	\left(
		x-\frac{c\,x^2}{(1+c^2)^2}-x
	\right)\,
=	&\\&
=	\lim_{x\to0^+}\frac{c}{(1+c^2)^2}
=	\frac{0}{(1+0^2)^2} = 0
&
\end{flalign*}
\end{sectionBox}

\end{multicols}












