% !TEX root = ./AM3C-Slides_annotations.0.tex
\documentclass["AM3C-Slides_annotations.tex"]{subfiles}

% \tikzset{external/force remake=true} % - remake all

\begin{document}

% \graphicspath{{\subfix{./.build/figures/AM3C-Slides_annotations.0}}}
% \tikzsetexternalprefix{./.build/figures/AM3C-Slides_annotations.0/graphics/}

\mymakesubfile{0}[AM 3C]
{Apendice} % Subfile Title
{Apendice} % Part Title

\begin{sectionBox}1{Identidades Trigonométricas} % S2
  \begin{multicols}{2}
    \begin{align}
        \sin^2(x) + \cos^2(x) &= 1
      \\ 1 + \tan^2(x)         &= \sec^2(x)
      \\ 1 + \cot^2(x)         &= \csc^2(x)
    \end{align}
    \begin{align}
         \sin^2(x)             &= \frac{1-\cos(2\,x)}{2}
      \\ \cos^2(x)             &= \frac{1+\cos(2\,x)}{2}
      \\ \sin(2x)              &= 2 \sin(x)\,\cos(x)
    \end{align}
  \end{multicols}
  \begin{align}
       2\,\sin(x)\,\cos(y)   &= \sin(x - y) + \sin(x + y)
    \\ 2\,\sin(x)\,\sin(y)   &= \cos(x - y) - \cos(x + y)
    \\ \cos(x)\,\cos(y)      &= \cos(x - y) + \cos(x + 1)
    \\ 1 \pm \sin(x)           &= 1 \pm \cos(\pi/2 - x)
  \end{align}
\end{sectionBox}

\begin{sectionBox}1{Trigonometria Hiperbólica} % S3
  \begin{multicols}{2}
    \begin{align}
         \sinh(x) &= \frac{e^{x}-e^{-x}}{2}
      \\ \cosh(x) &= \frac{e^{x}+e^{-x}}{2}
      \\ \tanh(x) &= \frac{\sinh(x)}{\cosh(x)}=\frac{e^{x}-e^{-x}}{e^{x}+e^{-x}}
    \end{align}
    \begin{align}
         \coth(x) &= 1/\tanh(x)
      \\ \sech(x) &= 1/\cosh(x)
      \\ \csch(x) &= 1/\sinh(x)
    \end{align}
  \end{multicols}
\end{sectionBox}

\begin{sectionBox}1{Tabela de Derivadas} % S4
  \begin{multicols}{2}

    \subsection*{Basic}
    \begin{align}
      % Basic
        \left(u^n\right)'     &= n\,u^{n-1}\,u'
      \\ \left(u\phantom{/}v\right)' &= \phantom{(}u'\,v + v'\,u
      \\ \left(u/v\right)'    &=   \left(  u'\,v - v'\,u\right)/v^2
    \end{align}

    \subsection*{Exponentials}
    \begin{align}
      % exponentials
         \left(a^u\right)'&= a^u\,\ln(a)\,u'; \qquad (a>0 \land a\neq1) 
      \\ \left(e^u\right)'&= e^u\,u' 
      \\ \log'_{a} (u)    &= \frac{u'}{u}\,\log_{a}(e) 
      \\ \ln'(u)          &= \frac{1}{u}\,u' 
      \\ (u^v)'           &= v\,u^{v-1}\,u' + u^v\,\ln(u)\,v' 
    \end{align}

    \subsection*{Trigonométric}
    \begin{align}
      % trigonometric
         \sin'(u)&= \phantom{-}u'\,\cos(u) 
      \\ \cos'(u)&=   - u'\,\sin(u) 
      \\ \tan'(u)&= \phantom{-}u'\,\sec^2(u) 
      \\ \cot'(u)&=   - u'\,\csc^2(u) 
      \\ \sec'(u)&= \phantom{-}u'\,\sec(u)\,\tan(u) 
      \\ \csc'(u)&=   - u'\,\csc(u)\,\cot(u) 
    \end{align}

    \subsection*{Hyperbolic}
    \begin{align}
      % hyperbolic
        \sinh'(u)&= \cosh(u) 
      \\ \cosh'(u)&= \sinh(u) 
      \\ \tanh'(u)&= 1-\tanh^2(u) 
      \\ \coth'(u)&= 1-\coth^2(u) 
      \\ \sech'(u)&= -\tanh(u)\,\sech(u) 
      \\ \csch'(u)&= -\coth(u)\,\csch(u) 
    \end{align}

    \subsection*{Arcs}
    \begin{align}
      % arcs
        \arcsin'(u)&= \phantom{-}\frac{u'}{\sqrt{1-u^2}} 
      \\ \arccos'(u)&=           -\frac{u'}{\sqrt{1-u^2}} 
      \\ \arctan'(u)&= \phantom{-}\frac{u'}{1+u^2}  
      \\ \arccot'(u)&=           -\frac{u'}{1+u^2}  
      \\ \arcsec'(u)&= \phantom{-}\frac{u'}{|u|\,\sqrt{u^2-1}};(|u| > 1) 
      \\ \arccsc'(u)&=           -\frac{u'}{|u|\,\sqrt{u^2-1}};(|u| > 1) 
    \end{align} 

  \end{multicols}
\end{sectionBox}

\begin{sectionBox}1{Tabela de Integrais} % S6
  \subsection*{Basics}
  \begin{align}
       \int       \odif{u}    &= c + u 
    \\ \int   u^n \odif{u}    &= c + \frac{u^{n+1}}{n+1} ;& (n \neq -1) 
    \\ \int \odif{u}/u        &= c + \ln\myvert{u}
    \\ \int   a^u \odif{u}    &= c + \frac{a^u}{\ln{a}} ;& (a > 0 \land a \neq 1)
    \\ \int   e^u \odif{u}    &= c + e^u
  \end{align}

  \subsection*{trigonometric}
  % \begin{multicols}{1}
    \begin{align}
         \int \sin(u)\,         \odif{u}&= c - \cos{u}
      \\ \int \cos(u)\,         \odif{u}&= c + \sin{u}
      \\ \int \tan(u)\,         \odif{u}&= c + \ln|\sec(u)          |
      \\ \int \cot(u)\,         \odif{u}&= c + \ln|\sin(u)          |
      \\ \int \sec(u)\,         \odif{u}&= c + \ln|\sec(u) + \tan(u)|
      \\ \int \csc(u)\,         \odif{u}&= c + \ln|\csc(u) - \cot(u)|
      \\ \int \sec(u)\,\tan(u)\,\odif{u}&= c + \sec(u)
      \\ \int \csc(u)\,\cot(u)\,\odif{u}&= c - \csc(u)
      \\ \int \sec^2(u)\,       \odif{u}&= c + \tan(u)
      \\ \int \csc^2(u)\,       \odif{u}&= c - \cot(u)
    \end{align}
  % \end{multicols}
  \subsection*{expressions}
  \begin{align}
       \int \odif{u}/     (u^2 + a^2) &= \arctan(u/a)/a + c 
    \\ \int \odif{u}/     (u^2 - a^2) &= \ln\left|\frac{u-a}{u+a}\right|/2\,a + c ;& (u^2 > a^2) 
    \\ \int \odif{u}/    \sqrt{u^2 + a^2} &= \ln{|u + \sqrt{u^2+a^2}|} + c 
    \\ \int \odif{u}/    \sqrt{u^2 - a^2} &= \arcsin(u/a) + c ;& (u^2 < a^2) 
    \\ \int \odif{u}/    \sqrt{a^2 - u^2} &= \arcsin(u/a) + c ;& (u^2 < a^2) 
    \\ \int \odif{u}/\left(u\,\sqrt{a^2 - u^2}\right)&= \arcsec|u/a|/a + c  
  \end{align}

  \subsection*{Uncommon Integrals}
  \begin{align}
    \int{\sin^n(a\,u)\,\odif{u}}
    &= 
    - \frac
    { \sin^{n-1}(a\,u)\,\cos(a\,u)}
    {a\,n}
    + \frac{n-1}{n}
    \,\int{\sin^{n-2}(a\,u)\,\odif{u}}
    % 
    % 
    % 
    \\
    \int{\cos^n(a\,u)\,\odif{u}}
    &= \phantom{-} 
    \frac
    { \sin(a\,u)\,\cos^{n-1}(a\,u)}
    {a\,n}
    +\frac{n-1}{n}
    \,\int{\cos^{n-2}(a\,u)\,\odif{u}}
    %
    %
    %
    \\
    \int{\tan^n(a\,u)\,\odif{u}}
    &= \phantom{-} 
    \frac
    { \tan^{n-1}(a\,u) }
    {a(n-1)}
    -\int{\tan^{n-2}(a\,u)\,\odif{u}}
    %
    %
    %
    \\
    \int{\cot^n(a\,u)\,\odif{u}}
    &=
    - \frac
    {\cot^{n-1}(a\,u)}
    {a(n-1)}
    -\int{\cot^{n-2}(a\,u)\,\odif{u}}
    %
    %
    %
    \\
    \int{\sec^n(a\,u)\,\odif{u}}
    &= \phantom{-}
    \frac
    {\sec^{n-2}(a\,u) \tan(a\,u)}
    {a\,(n-1)}
    + \frac{n-2}{n-1}
    \,\int{\sec^{n-2}(a\,u)\,\odif{u}}
    %
    %
    %
    \\
    \int{\csc^n(a\,u)\,\odif{u}}
    &=
    - \frac
    {\csc^{n-2}(a\,u) \cot(a\,u)}
    {a\,(n-1)}
    + \frac{n-2}{n-1}
    \,\int{\csc^{n-2}(a\,u)\,\odif{u}}
  \end{align}

  \subsection*{Indefinite Integral Rules}
  \begin{align}
    P(u\,v') &= u\,v - P(u'\,v)
    \\ P(f(g(x))\,g'(x)) &= P(f(u)\,\odif{u});\quad u = g(x)
  \end{align}
  
\end{sectionBox}

\end{document}
